\documentclass{report}

\usepackage{amsmath, amsfonts, amsthm}
\usepackage[scale = 0.8]{geometry}

\begin{document}
    \section*{Problem 1}
    Let $S_n(x) = \sum_{k=1}^n f_k(x)$. For $m \ge n$,
    \begin{align*}
        \sum_{k=1}^m f_k g_k - \sum_{k=1}^n f_k g _k &= \sum_{k=n}^{m-1}S_k(g_k-g_{k+1})
            + (S_m g_m - S_n g_n) 
    \end{align*}
    Since $|S_n| \le C$ for $n \in \mathbb{N}$ and $g_k - g_{k+1} \ge 0$ for any 
    $k \in \mathbb{N}$, we have:
    \begin{align*}
        \left| \sum_{k=1}^m f_k g_k\right| \le \sum_{k=n}^{m-1} C (g_k-g_{k+1}) + 
            C(g_m - g_n) = 2Cg_n
    \end{align*}
    Since $g_n$ converges uniformly on $E$ to 0, for any $\varepsilon > 0$, there 
    exist $N(\varepsilon)$ such that for $n \ge N$, we have $g_n<\frac{\varepsilon}{2C}$.
    Thus we conclude that for $N \le n \le m$, 
    \begin{align*}
        \left| \sum_{k=1}^m f_k g_k\right|
    \end{align*}
\end{document}